$`\leftrightarrow \neq(x\ y)\lnot=(x\ y)`$\
$`\leftrightarrow \notin(x\ y)\lnot\in(x\ y)`$\
$`\leftrightarrow \subseteq(x\ y)\forall t\rightarrow\in(t\ x)\in(t\ y)`$\
$`\leftrightarrow \subset(x\ y)\land\subseteq(x\ y)\neq(x\ y)`$\
$`\leftrightarrow =(\emptyset\ y)\forall t\notin(t\ \emptyset)`$\
$`\leftrightarrow =(\cap(x\ y)\ z)\forall t\leftrightarrow \in(t\ z)\land\in(t\ x)\in(t\ y)`$\
$`\leftrightarrow =(\cup(x\ y)\ z)\forall t\leftrightarrow \in(t\ z)\lor\in(t\ x)\in(t\ y)`$\
$`\leftrightarrow =(\sim(x\ y)\ z)\forall t\leftrightarrow \in(t\ z)\land\in(t\ x)\notin(t\ y)`$\
$`\leftrightarrow =(\bigcap(x)\ y)\land\rightarrow\neq(x\ \emptyset)\forall t\leftrightarrow\in(t\ y)\forall z\rightarrow\in(z\ x)\in(t\ z)\rightarrow=(x\ \emptyset)=(y\ \emptyset)`$\
$`\leftrightarrow =(\bigcup(x)\ y)\forall t\leftrightarrow \in(t\ y)\exists z\land\in(t\ z)\in(z\ x)`$\
$`\leftrightarrow=(power(x)\ y)\forall t\leftrightarrow\in(t\ y)\subseteq(t\ x)`$\
$`\leftrightarrow=(pair(x\ y)\ z)\forall t\leftrightarrow\in(t\ z)\land=(t\ x)=(t\ y)`$\
$`=(the(x)\ pair(x\ x)`$\
$`=(tuple(x\ y)\ pair(the(x)\ pair(x\ y))`$\
$`\leftrightarrow=(\times(x\ y)\ z)\forall t`$
